Refactor `par` and repair substitutions

Semantic/CoreCapybara/Substitution.lean
@@ -124,7 +124,7 @@ def Exp.subst : Exp s1 -> Subst s1 s2 -> Exp s2
 | .read x, s => .read (x.subst s)
 | .write x y, s => .write (x.subst s) (y.subst s)
 | .cond x e2 e3, s => .cond (x.subst s) (e2.subst s) (e3.subst s)
-| .par e1 e2, s => .par (e1.subst s) (e2.subst s)
+| .par C1 C2 e1 e2, s => .par (C1.subst s) (C2.subst s) (e1.subst s) (e2.subst s)
 
 /-- Substitution that opens a variable binder by replacing the innermost bound variable with `x`. -/
 def Subst.openVar (x : Var .var s) : Subst (s,x) s where
@@ -624,8 +624,8 @@ theorem Exp.subst_comp {e : Exp s1} {σ1 : Subst s1 s2} {σ2 : Subst s2 s3} :
   | write x y => simp only [Exp.subst, Var.subst_comp]
   | cond x e2 e3 ih2 ih3 =>
     simp only [Exp.subst, Var.subst_comp, ih2, ih3]
-  | par e1 e2 ih1 ih2 =>
-    simp only [Exp.subst, ih1, ih2]
+  | par C1 C2 e1 e2 ih1 ih2 =>
+    simp only [Exp.subst, CaptureSet.subst_comp, ih1, ih2]
 
 /-- Substitution on separation contexts distributes over composition of substitutions. -/
 theorem SepCtx.subst_comp {K : SepCtx s1} {σ1 : Subst s1 s2} {σ2 : Subst s2 s3} :
@@ -784,8 +784,8 @@ theorem Exp.subst_id {e : Exp s} :
     simp only [Exp.subst, Var.subst_id]
   | cond x e2 e3 ih2 ih3 =>
     simp only [Exp.subst, Var.subst_id, ih2, ih3]
-  | par e1 e2 ih1 ih2 =>
-    simp only [Exp.subst, ih1, ih2]
+  | par C1 C2 e1 e2 ih1 ih2 =>
+    simp only [Exp.subst, CaptureSet.subst_id, ih1, ih2]
 
 /-- Substituting with the identity substitution leaves a separation context unchanged. -/
 theorem SepCtx.subst_id {K : SepCtx s} :
@@ -966,8 +966,8 @@ theorem Exp.subst_asSubst {e : Exp s1} {f : Rename s1 s2} :
     simp only [Exp.subst, Exp.rename, Var.subst_asSubst]
   | cond x e2 e3 ih2 ih3 =>
     simp only [Exp.subst, Exp.rename, Var.subst_asSubst, ih2, ih3]
-  | par e1 e2 ih1 ih2 =>
-    simp only [Exp.subst, Exp.rename, ih1, ih2]
+  | par C1 C2 e1 e2 ih1 ih2 =>
+    simp only [Exp.subst, Exp.rename, CaptureSet.subst_asSubst, ih1, ih2]
 
 /-- Substituting a substitution lifted from a renaming is the same as renaming. -/
 theorem SepCtx.subst_asSubst {K : SepCtx s1} {f : Rename s1 s2} :
@@ -1362,10 +1362,11 @@ def Exp.is_closed_subst {e : Exp s1} {σ : Subst s1 s2}
     cases hc with | cond hx h2 h3 =>
     simp only [Exp.subst]
     exact IsClosed.cond (Var.is_closed_subst hx hsubst) (ih2 h2 hsubst) (ih3 h3 hsubst)
-  | par e1 e2 ih1 ih2 =>
-    cases hc with | par h1 h2 =>
+  | par C1 C2 e1 e2 ih1 ih2 =>
+    cases hc with | par hc1 hc2 h1 h2 =>
     simp only [Exp.subst]
-    exact IsClosed.par (ih1 h1 hsubst) (ih2 h2 hsubst)
+    exact IsClosed.par (CaptureSet.is_closed_subst hc1 hsubst)
+      (CaptureSet.is_closed_subst hc2 hsubst) (ih1 h1 hsubst) (ih2 h2 hsubst)
 
 /-- The openVar substitution is closed if the variable is closed. -/
 theorem Subst.openVar_is_closed {z : Var .var s}
@@ -1601,9 +1602,10 @@ theorem Exp.subst_closed_inv {e : Exp s1} {σ : Subst s1 s2}
     simp only [Exp.subst] at hclosed
     cases hclosed with | cond hx h2 h3 =>
     exact IsClosed.cond (Var.subst_closed_inv hx) (ih2 h2) (ih3 h3)
-  | par e1 e2 ih1 ih2 =>
+  | par C1 C2 e1 e2 ih1 ih2 =>
     simp only [Exp.subst] at hclosed
-    cases hclosed with | par h1 h2 =>
-    exact IsClosed.par (ih1 h1) (ih2 h2)
+    cases hclosed with | par hc1 hc2 h1 h2 =>
+    exact IsClosed.par (CaptureSet.subst_closed_inv hc1) (CaptureSet.subst_closed_inv hc2)
+      (ih1 h1) (ih2 h2)
 
 end CoreCapybara
